theories/Spilling/RepairSpillInv.v
@@ -1,14 +1,42 @@
-Require Import RepairSpill.
+Require Import RepairSpill RegLive.
 Require Import SpillSound Annotation Liveness.Liveness.
-Require Import List Map IL.
+Require Import List Map IL Take TakeSet OneOrEmpty.
 
 Set Implicit Arguments.
 
 (** * Invariance on correct spillings *)
 
 (* assumptions missing *)
-Lemma repair_spill_inv
+Lemma repair_spill_inv k ZL Λ s lv sl R M G
   : live_sound Imperative ZL (merge ⊝ Λ) s lv
     -> spill_sound k ZL Λ (R,M) s sl
-    -> sl === repair_spill k ZL Λ R M s lv sl
+    -> sl === repair_spill k ZL Λ R M s lv (reg_live (fst ⊝ Λ) ZL G s sl) sl
 .
+Proof.
+  intros liveSnd spillSnd.
+  general induction sl; invc liveSnd; invc spillSnd; econstructor.
+  - econstructor; econstructor; symmetry;
+      apply inter_subset_equal in H9; apply inter_subset_equal in H10.
+    + rewrite H9; erewrite !get_nth; eauto. unfold snd. apply union_subset_equal.
+      rewrite H17. clear; cset_tac.
+    + erewrite !get_nth; eauto. rewrite H9, H10. unfold fst. apply union_subset_equal.
+      rewrite H16. clear; cset_tac.
+    + erewrite !get_nth; eauto. unfold snd, fst. econstructor; eauto.
+      apply union_subset_equal. rewrite H17. unfold set_take; rewrite take_set_incl. admit. (*
+      rewrite meet_comm. apply meet_incl. rewrite H18. cset_tac. rewrite H16.
+      apply incl_eq.
+      * admit.
+      * rewrite H17. apply union_incl_split.
+        -- clear; cset_tac.
+        -- rewrite H9 at 2. rewrite H10. unfold set_take. rewrite take_set_incl.
+           rewrite H18. rewrite H16.*)
+
+    + econstructor; eauto.      
+  - econstructor; econstructor; symmetry; apply inter_subset_equal in H6;
+      eauto.
+    apply inter_subset_equal in H7. rewrite H6, H7. apply union_subset_equal.
+    clear - H8. cset_tac.
+  - econstructor; econstructor; symmetry;
+      apply inter_subset_equal in H12; apply inter_subset_equal in H13.
+    + rewrite H12 at 6. apply union_subset_equal. admit. 
+    + rewrite H12, H13. apply union_subset_equal. clear - H15; cset_tac.
